plugin/tests/test_extract.v
@@ -15,6 +15,7 @@ MetaCoq Extract Module compile "compile.mlf".
 
 From Malfunction Require Import Pipeline.
 MetaCoq Extract Module compile_malfunction "compile_malfunction.mlf".
+
 (* 
 MetaCoq Quote Recursively Definition tm := compile_malfunction.
 
